@prefix rdf: <http://www.w3.org/1999/02/22-rdf-syntax-ns#> .
@prefix rdfs: <http://www.w3.org/2000/01/rdf-schema#> .
@prefix skos: <http://www.w3.org/2004/02/skos/core#> .
@prefix owl: <http://www.w3.org/2002/07/owl#> .
@prefix dcterms: <http://purl.org/dc/terms/> .
@prefix ddicv-sumstats: <http://rdf-vocabulary.ddialliance.org/DDICV/SummaryStatisticsType_1.0#> .

ddicv-sumstats:CodeList a skos:ConceptScheme ;
	dcterms:title "Summary Statistic Type"@en ;
	skos:notation "SummaryStatisticsType" ;
	dcterms:description "Specifies the type of summary statistic. Summary statistics are a single number representation of the characteristics of a set of values."@en ;
	dcterms:isVersionOf <http://rdf-vocabulary.ddialliance.org/DDICV/SummaryStatisticsType#> ;
	owl:versionInfo "1.0" ;
	skos:hasTopConcept ddicv-sumstats:ArithmeticMean , ddicv-sumstats:GeometricMean , ddicv-sumstats:HarmonicMean , ddicv-sumstats:TrimmedMean , ddicv-sumstats:StandardErrorOfMean , ddicv-sumstats:Mode , ddicv-sumstats:Median , ddicv-sumstats:ValidCases , ddicv-sumstats:InvalidCases , ddicv-sumstats:Minimum , ddicv-sumstats:Maximum , ddicv-sumstats:Range , ddicv-sumstats:Sum , ddicv-sumstats:Variance , ddicv-sumstats:StandardDeviation , ddicv-sumstats:CoefficientOfVariation , ddicv-sumstats:AverageAbsoluteDeviation , ddicv-sumstats:MedianAbsoluteDeviation , ddicv-sumstats:FirstQuartile , ddicv-sumstats:SecondQuartile , ddicv-sumstats:ThirdQuartile , ddicv-sumstats:InterquartileRange , ddicv-sumstats:FirstQuintile , ddicv-sumstats:SecondQuintile , ddicv-sumstats:ThirdQuintile , ddicv-sumstats:FourthQuintile , ddicv-sumstats:InterquintileRange , ddicv-sumstats:FirstDecile , ddicv-sumstats:SecondDecile , ddicv-sumstats:ThirdDecile , ddicv-sumstats:FourthDecile , ddicv-sumstats:FifthDecile , ddicv-sumstats:SixthDecile , ddicv-sumstats:SeventhDecile , ddicv-sumstats:EighthDecile , ddicv-sumstats:NinthDecile , ddicv-sumstats:InterdecileRange , ddicv-sumstats:OtherPercentile , ddicv-sumstats:Beta1 , ddicv-sumstats:Beta2 , ddicv-sumstats:ShapiroWilk , ddicv-sumstats:Other ;
	dcterms:license <http://creativecommons.org/licenses/by-sa/3.0/> ;
	dcterms:rights "Copyright DDI Alliance 2011" .

ddicv-sumstats:ArithmeticMean a skos:Concept ;
	skos:inScheme ddicv-sumstats:CodeList ;
	skos:prefLabel "Arithmetic mean (X)"@en ;
	skos:notation "ArithmeticMean" ;
	skos:definition "Mathematical average of a set of values. The mean is calculated by adding up two or more values and dividing the total by their number. In social/political science, it is usually the sum of the measurements divided by the number of subjects, or cases."@en .

ddicv-sumstats:GeometricMean a skos:Concept ;
	skos:inScheme ddicv-sumstats:CodeList ;
	skos:prefLabel "Geometric mean"@en ;
	skos:notation "GeometricMean" ;
	skos:definition "Average value of all data if extracting the nth root of the product of all (n) values. Rarely used in social sciences."@en .

ddicv-sumstats:HarmonicMean a skos:Concept ;
	skos:inScheme ddicv-sumstats:CodeList ;
	skos:prefLabel "Harmonic mean"@en ;
	skos:notation "HarmonicMean" ;
	skos:definition "Average value of all data if calculating the reciprocal of the arithmetic mean of the reciprocal of values. Rarely used in social sciences."@en .

ddicv-sumstats:TrimmedMean a skos:Concept ;
	skos:inScheme ddicv-sumstats:CodeList ;
	skos:prefLabel "Trimmed mean"@en ;
	skos:notation "TrimmedMean" ;
	skos:definition "The (arithmetic) mean calculated after discarding given parts of observations at the high and low end (e.g., interquartile mean when the lowest 25% and the highest 25% are discarded, and the mean of the remaining values is calculated)."@en .

ddicv-sumstats:StandardErrorOfMean a skos:Concept ;
	skos:inScheme ddicv-sumstats:CodeList ;
	skos:prefLabel "Standard error of the mean"@en ;
	skos:notation "StandardErrorOfMean" ;
	skos:definition "The Standard Error for the mean value."@en .

ddicv-sumstats:Mode a skos:Concept ;
	skos:inScheme ddicv-sumstats:CodeList ;
	skos:prefLabel "Mode (Mo)"@en ;
	skos:notation "Mode" ;
	skos:definition "The most frequently observed data value (Statistics Canada)."@en .

ddicv-sumstats:Median a skos:Concept ;
	skos:inScheme ddicv-sumstats:CodeList ;
	skos:prefLabel "Median (Mdn)"@en ;
	skos:notation "Median" ;
	skos:definition "The values below which, and above which, half of the values in a distribution fall (50th percentile)."@en .

ddicv-sumstats:ValidCases a skos:Concept ;
	skos:inScheme ddicv-sumstats:CodeList ;
	skos:prefLabel "Valid Cases"@en ;
	skos:notation "ValidCases" ;
	skos:definition "Cases with observations which are considered to be valid, i.e., providing substantial information and to be included for calculation."@en .

ddicv-sumstats:InvalidCases a skos:Concept ;
	skos:inScheme ddicv-sumstats:CodeList ;
	skos:prefLabel "Invalid cases"@en ;
	skos:notation "InvalidCases" ;
	skos:definition "Cases which are considered/defined as missing (e.g., not ascertained, not applicable, etc.), usually excluded from calculation."@en .

ddicv-sumstats:Minimum a skos:Concept ;
	skos:inScheme ddicv-sumstats:CodeList ;
	skos:prefLabel "Minimum"@en ;
	skos:notation "Minimum" ;
	skos:definition "The lowest valid value in a variable."@en .

ddicv-sumstats:Maximum a skos:Concept ;
	skos:inScheme ddicv-sumstats:CodeList ;
	skos:prefLabel "Maximum"@en ;
	skos:notation "Maximum" ;
	skos:definition "The highest valid value in a variable."@en .

ddicv-sumstats:Range a skos:Concept ;
	skos:inScheme ddicv-sumstats:CodeList ;
	skos:prefLabel "Range"@en ;
	skos:notation "Range" ;
	skos:definition "The range of valid values, i.e., all values that fall between the lowest and highest valid values."@en .

ddicv-sumstats:Sum a skos:Concept ;
	skos:inScheme ddicv-sumstats:CodeList ;
	skos:prefLabel "Sum"@en ;
	skos:notation "Sum" ;
	skos:definition "The sum or total of the values, across all valid cases."@en .

ddicv-sumstats:Variance a skos:Concept ;
	skos:inScheme ddicv-sumstats:CodeList ;
	skos:prefLabel "Variance (s2)"@en ;
	skos:notation "Variance" ;
	skos:definition "The variance is the mean square deviation of the variable around the average value. It reflects the dispersion of a frequency distribution around its mean (OECD Glossary of Statistics)."@en .

ddicv-sumstats:StandardDeviation a skos:Concept ;
	skos:inScheme ddicv-sumstats:CodeList ;
	skos:prefLabel "Standard deviation (s)"@en ;
	skos:notation "StandardDeviation" ;
	skos:definition "The positive square root of the variance. The most widely used measure of dispersion of a frequency distribution."@en .

ddicv-sumstats:CoefficientOfVariation a skos:Concept ;
	skos:inScheme ddicv-sumstats:CodeList ;
	skos:prefLabel "Coefficient of variation (CV)"@en ;
	skos:notation "CoefficientOfVariation" ;
	skos:definition "Standard deviation divided by the mean."@en .

ddicv-sumstats:AverageAbsoluteDeviation a skos:Concept ;
	skos:inScheme ddicv-sumstats:CodeList ;
	skos:prefLabel "Average absolute deviation (AAD)"@en ;
	skos:notation "AverageAbsoluteDeviation" ;
	skos:definition "The average of the absolute differences between each value and the overall mean. Measure of statistical dispersion around the mean, alternative to Standard Deviation."@en .

ddicv-sumstats:MedianAbsoluteDeviation a skos:Concept ;
	skos:inScheme ddicv-sumstats:CodeList ;
	skos:prefLabel "Median absolute deviation (MAD)"@en ;
	skos:notation "MedianAbsoluteDeviation" ;
	skos:definition "The median absolute deviation from the median. Measure of statistical dispersion around the median."@en .

ddicv-sumstats:FirstQuartile a skos:Concept ;
	skos:inScheme ddicv-sumstats:CodeList ;
	skos:prefLabel "First quartile"@en ;
	skos:notation "FirstQuartile" ;
	skos:definition "The first of three values which separate the total frequency of a distribution into four equal parts."@en .

ddicv-sumstats:SecondQuartile a skos:Concept ;
	skos:inScheme ddicv-sumstats:CodeList ;
	skos:prefLabel "Second quartile"@en ;
	skos:notation "Second Quartile" ;
	skos:definition "The second of three values which separate the total frequency of a distribution into four equal parts (= median)."@en .

ddicv-sumstats:ThirdQuartile a skos:Concept ;
	skos:inScheme ddicv-sumstats:CodeList ;
	skos:prefLabel "Third quartile"@en ;
	skos:notation "ThirdQuartile" ;
	skos:definition "The third of three values which separate the total frequency of a distribution into four equal parts."@en .

ddicv-sumstats:InterquartileRange a skos:Concept ;
	skos:inScheme ddicv-sumstats:CodeList ;
	skos:prefLabel "Interquartile range"@en ;
	skos:notation "InterquartileRange" ;
	skos:definition "The range between the first and third quartile values."@en .

ddicv-sumstats:FirstQuintile a skos:Concept ;
	skos:inScheme ddicv-sumstats:CodeList ;
	skos:prefLabel "First quintile"@en ;
	skos:notation "FirstQuintile" ;
	skos:definition "The first of four values which separate the total frequency of a distribution into five equal parts."@en .

ddicv-sumstats:SecondQuintile a skos:Concept ;
	skos:inScheme ddicv-sumstats:CodeList ;
	skos:prefLabel "Second quintile"@en ;
	skos:notation "SecondQuintile" ;
	skos:definition "The second of four values which separate the total frequency of a distribution into five equal parts."@en .

ddicv-sumstats:ThirdQuintile a skos:Concept ;
	skos:inScheme ddicv-sumstats:CodeList ;
	skos:prefLabel "Third quintile"@en ;
	skos:notation "ThirdQuintile" ;
	skos:definition "The third of four values which separate the total frequency of a distribution into five equal parts."@en .

ddicv-sumstats:FourthQuintile a skos:Concept ;
	skos:inScheme ddicv-sumstats:CodeList ;
	skos:prefLabel "Fourth quintile"@en ;
	skos:notation "FourthQuintile" ;
	skos:definition "The fourth of four values which separate the total frequency of a distribution into five equal parts."@en .

ddicv-sumstats:InterquintileRange a skos:Concept ;
	skos:inScheme ddicv-sumstats:CodeList ;
	skos:prefLabel "Interquintile range"@en ;
	skos:notation "InterquintileRange" ;
	skos:definition "The range between the first and fourth quintile values."@en .

ddicv-sumstats:FirstDecile a skos:Concept ;
	skos:inScheme ddicv-sumstats:CodeList ;
	skos:prefLabel "First decile"@en ;
	skos:notation "FirstDecile" ;
	skos:definition "The first of nine values which separate the total frequency of a distribution into ten equal parts."@en .

ddicv-sumstats:SecondDecile a skos:Concept ;
	skos:inScheme ddicv-sumstats:CodeList ;
	skos:prefLabel "Second decile"@en ;
	skos:notation "SecondDecile" ;
	skos:definition "The second of nine values which separate the total frequency of a distribution into ten equal parts."@en .

ddicv-sumstats:ThirdDecile a skos:Concept ;
	skos:inScheme ddicv-sumstats:CodeList ;
	skos:prefLabel "Third decile"@en ;
	skos:notation "ThirdDecile" ;
	skos:definition "The third of nine values which separate the total frequency of a distribution into ten equal parts."@en .

ddicv-sumstats:FourthDecile a skos:Concept ;
	skos:inScheme ddicv-sumstats:CodeList ;
	skos:prefLabel "Fourth decile"@en ;
	skos:notation "FourthDecile" ;
	skos:definition "The fourth of nine values which separate the total frequency of a distribution into ten equal parts."@en .

ddicv-sumstats:FifthDecile a skos:Concept ;
	skos:inScheme ddicv-sumstats:CodeList ;
	skos:prefLabel "Fifth decile"@en ;
	skos:notation "FifthDecile" ;
	skos:definition "The fifth of nine values which separate the total frequency of a distribution into ten equal parts (= median)."@en .

ddicv-sumstats:SixthDecile a skos:Concept ;
	skos:inScheme ddicv-sumstats:CodeList ;
	skos:prefLabel "Sixth decile"@en ;
	skos:notation "SixthDecile" ;
	skos:definition "The sixth of nine values which separate the total frequency of a distribution into ten equal parts."@en .

ddicv-sumstats:SeventhDecile a skos:Concept ;
	skos:inScheme ddicv-sumstats:CodeList ;
	skos:prefLabel "Seventh decile"@en ;
	skos:notation "SeventhDecile" ;
	skos:definition "The seventh of nine values which separate the total frequency of a distribution into ten equal parts."@en .

ddicv-sumstats:EighthDecile a skos:Concept ;
	skos:inScheme ddicv-sumstats:CodeList ;
	skos:prefLabel "Eighth decile"@en ;
	skos:notation "EighthDecile" ;
	skos:definition "The eighth of nine values which separate the total frequency of a distribution into ten equal parts."@en .

ddicv-sumstats:NinthDecile a skos:Concept ;
	skos:inScheme ddicv-sumstats:CodeList ;
	skos:prefLabel "Ninth decile"@en ;
	skos:notation "NinthDecile" ;
	skos:definition "The ninth of nine values which separate the total frequency of a distribution into ten equal parts."@en .

ddicv-sumstats:InterdecileRange a skos:Concept ;
	skos:inScheme ddicv-sumstats:CodeList ;
	skos:prefLabel "Interdecile range"@en ;
	skos:notation "InterdecileRange" ;
	skos:definition "The range between the first and ninth decile values."@en .

ddicv-sumstats:OtherPercentile a skos:Concept ;
	skos:inScheme ddicv-sumstats:CodeList ;
	skos:prefLabel "Other percentile"@en ;
	skos:notation "OtherPercentile" ;
	skos:definition "A percentile not covered by any of the other percentile terms."@en .

ddicv-sumstats:Beta1 a skos:Concept ;
	skos:inScheme ddicv-sumstats:CodeList ;
	skos:prefLabel "Skewness"@en ;
	skos:notation "Beta1" ;
	skos:definition "A measure for the asymmetry of a probability distribution of a variable."@en .

ddicv-sumstats:Beta2 a skos:Concept ;
	skos:inScheme ddicv-sumstats:CodeList ;
	skos:prefLabel "Kurtosis"@en ;
	skos:notation "Beta2" ;
	skos:definition "A measure for the peakedness of a probability distribution of a variable."@en .

ddicv-sumstats:ShapiroWilk a skos:Concept ;
	skos:inScheme ddicv-sumstats:CodeList ;
	skos:prefLabel "Shapiro-Wilk"@en ;
	skos:notation "ShapiroWilk" ;
	skos:definition "Normality test statistics."@en .

ddicv-sumstats:Other a skos:Concept ;
	skos:inScheme ddicv-sumstats:CodeList ;
	skos:prefLabel "Other"@en ;
	skos:notation "Other" ;
	skos:definition "Use if the summary statistic type is known, but not found in the list."@en .
